Introduce value preservation lemma for the DELEGS subsystem

Isabelle/Shelley/Delegation.thy
@@ -1,36 +1,16 @@
 section \<open> Delegation \<close>
 
 theory Delegation
-  imports Finite_Map_Extras Basic_Types Address
+  imports Finite_Map_Extras Basic_Types Address Delegation_Certificates Transaction
 begin
-
-subsection \<open> Delegation Definitions \<close>
-
-text \<open> Delegation certificate \<close>
-
-datatype d_cert = DCert_RegKey | DCert_DeregKey \<comment> \<open>NOTE: Incomplete for now\<close>
-
-text \<open> Registered stake credential \<close>
-
-typedecl stake_creds \<comment> \<open>NOTE: Abstract for now\<close>
-
-text \<open> Registered stake pools \<close>
-
-typedecl stake_pools \<comment> \<open>NOTE: Abstract for now\<close>
-
-text \<open> Certificate witness \<close>
-
-consts cwitness :: "d_cert \<Rightarrow> credential" \<comment> \<open>NOTE: Abstract for now\<close>
-
-text \<open> Registered credential \<close>
-
-consts reg_cred :: "d_cert \<Rightarrow> credential" \<comment> \<open>NOTE: Abstract for now\<close>
 
 subsection \<open> Delegation Transitions \<close>
 
 text \<open> Delegation States \<close>
 
 type_synonym d_state = "(addr_rwd, coin) fmap" \<comment> \<open>NOTE: Only rewards for now\<close>
+
+typedecl p_state \<comment> \<open>NOTE: Abstract for now\<close>
 
 text \<open> Delegation Environment \<close>
 
@@ -40,8 +20,10 @@ subsection \<open> Delegation Rules \<close>
 
 text \<open> Delegation Inference Rules \<close>
 
-text \<open> NOTE:
-  Although \<open>addr_rwd hk \<notin> dom rewards \<Longleftrightarrow> hk \<notin> dom stkCreds\<close> is a property of the system,
+text \<open>
+  NOTE:
+  \<^item> Only the \<open>deleg_reg\<close> and \<open>deleg_dereg\<close> rules are included for now.
+  \<^item> Although \<open>addr_rwd hk \<notin> dom rewards \<Longleftrightarrow> hk \<notin> dom stkCreds\<close> is a property of the system,
   it cannot be proven in \<open>DELEG\<close> alone (but possibly in \<open>DELEGS\<close>). So I had either to add an extra
   precondition \<open>addr_rwd hk \<notin> dom rewards\<close> or use \<open>\<union>\<^sub>\<leftarrow>\<close> instead of \<open>++\<^sub>f\<close> in rule \<open>deleg_reg\<close> since
   Lemma 15.6 is a property of \<open>DELEG\<close>.
@@ -59,5 +41,51 @@ inductive deleg_sts :: "d_env \<Rightarrow> d_state \<Rightarrow> d_cert \<Right
       if "c = DCert_DeregKey"
       and "hk = cwitness c"
       and "rewards $$ (addr_rwd hk) = Some 0"
+
+subsection \<open> Delegation and Pool Combined Rules \<close>
+
+text \<open> Delegation and Pool Combined Environment \<close>
+
+type_synonym d_p_env = slot \<comment> \<open>NOTE: Only slot for now\<close>
+
+text \<open> Delegation and Pool Combined State \<close>
+
+type_synonym d_p_state = "d_state \<times> p_state"
+
+text \<open> Delegation and Pool Combined Transition Rules \<close>
+
+text \<open>
+  NOTE:
+  \<^item> Only the \<open>delpl_deleg\<close> rule is included for now.
+\<close>
+inductive delpl_sts :: "d_p_env \<Rightarrow> d_p_state \<Rightarrow> d_cert \<Rightarrow> d_p_state \<Rightarrow> bool"
+  (\<open>_ \<turnstile> _ \<rightarrow>\<^bsub>DELPL\<^esub>{_} _\<close> [51, 0, 51] 50)
+  where
+    delpl_deleg: "
+      slot \<turnstile> (dstate, pstate) \<rightarrow>\<^bsub>DELPL\<^esub>{c} (dstate', pstate)"
+      if "slot \<turnstile> dstate \<rightarrow>\<^bsub>DELEG\<^esub>{c} dstate'"
+
+text \<open> Certificate Sequence Environment \<close>
+
+type_synonym d_p_s_env = "slot \<times> tx"
+
+text \<open> Delegation sequence rules \<close>
+
+text \<open>
+  NOTE:
+  \<^item> The first and second preconditions in the \<open>seq_delg_ind\<close> rule are not included for now.
+\<close>
+inductive delegs_sts :: "d_p_s_env \<Rightarrow> d_p_state \<Rightarrow> d_cert list \<Rightarrow> d_p_state \<Rightarrow> bool"
+  (\<open>_ \<turnstile> _ \<rightarrow>\<^bsub>DELEGS\<^esub>{_} _\<close> [51, 0, 51] 50)
+  where
+    seq_delg_base: "
+      (slot, tx) \<turnstile> (rewards, pstate) \<rightarrow>\<^bsub>DELEGS\<^esub>{[]} (rewards', pstate)"
+      if "wdrls = txwdrls tx"
+      and "wdrls \<subseteq>\<^sub>f rewards"
+      and "rewards' = rewards \<union>\<^sub>\<rightarrow> fmmap (\<lambda>_. 0) wdrls"
+    | seq_delg_ind: "
+      (slot, tx) \<turnstile> dpstate \<rightarrow>\<^bsub>DELEGS\<^esub>{\<Gamma> @ [c]} dpstate''"
+      if "(slot, tx) \<turnstile> dpstate \<rightarrow>\<^bsub>DELEGS\<^esub>{\<Gamma>} dpstate'"
+      and "slot \<turnstile> dpstate' \<rightarrow>\<^bsub>DELPL\<^esub>{c} dpstate''"
 
 end
