Isabelle/Shelley/Delegation_Certificates.thy
@@ -1,0 +1,29 @@
+section \<open> Delegation certificates \<close>
+
+theory Delegation_Certificates
+  imports Address
+begin
+
+subsection \<open> Delegation Definitions \<close>
+
+text \<open> Delegation certificate \<close>
+
+datatype d_cert = DCert_RegKey | DCert_DeregKey \<comment> \<open>NOTE: Incomplete for now\<close>
+
+text \<open> Registered stake credential \<close>
+
+typedecl stake_creds \<comment> \<open>NOTE: Abstract for now\<close>
+
+text \<open> Registered stake pools \<close>
+
+typedecl stake_pools \<comment> \<open>NOTE: Abstract for now\<close>
+
+text \<open> Certificate witness \<close>
+
+consts cwitness :: "d_cert \<Rightarrow> credential" \<comment> \<open>NOTE: Abstract for now\<close>
+
+text \<open> Registered credential \<close>
+
+consts reg_cred :: "d_cert \<Rightarrow> credential" \<comment> \<open>NOTE: Abstract for now\<close>
+
+end
